examples/unit-tests/bug21.fst
@@ -1,10 +1,21 @@
 module Bug21 
 
+val constfun0 : bool -> int -> Tot bool
+let constfun0 x k = x
+
+let ftrue0 = constfun0 true
+
+val test0 : int -> Tot unit
+let test0 x = assert (ftrue0 x = true)
+
 val constfun : 'a -> 'b -> Tot 'a
 let constfun x k = x
 
 val ftrue : 'b -> Tot bool
-let ftrue = constfun true 
+let ftrue = constfun true
+
+val test : int -> Tot unit
+let test x = assert (ftrue x = true)
 
 val my_override : ('a -> Tot 'b) -> 'a -> 'b -> Tot ('a -> Tot 'b)
 let my_override f k x k' = if k = k' then x else f k'
@@ -16,14 +27,14 @@ val override_example1 : unit -> Fact unit
       (ensures (fmostlytrue 0 = true))
 let override_example1 () = ()
 
-(* val override_example2 : unit -> Fact unit *)
-(*       (ensures (fmostlytrue 1 = false)) *)
-(* let override_example2 () = () *)
+val override_example2 : unit -> Fact unit
+      (ensures (fmostlytrue 1 = false))
+let override_example2 () = ()
 
-(* val override_example3 : unit -> Fact unit *)
-(*       (ensures (fmostlytrue 2 = true)) *)
-(* let override_example3 () = () *)
+val override_example3 : unit -> Fact unit
+      (ensures (fmostlytrue 2 = true))
+let override_example3 () = ()
 
-(* val override_example4 : unit -> Fact unit *)
-(*       (ensures (fmostlytrue 3 = false)) *)
-(* let override_example4 () = () *)
+val override_example4 : unit -> Fact unit
+      (ensures (fmostlytrue 3 = false))
+let override_example4 () = ()
